Stricter rules about that types need to be completely resolved. Renamed "default constructor" to "anonymous constructor" (since there's really nothing "default" about it). If the type of literal "null" is unresolved, make the type "object". The need to translate unresolved proxies is now assumed to be gone.

Source/Dafny/DafnyAst.cs
@@ -3332,7 +3332,7 @@ namespace Microsoft.Dafny {
   ///    Here, Path may either be of the form C.Init
   ///      -- represents new C.Init(EE)
   ///    or all of Path denotes a type
-  ///      -- represents new C._ctor(EE), where _ctor is the default constructor for class C
+  ///      -- represents new C._ctor(EE), where _ctor is the anonymous constructor for class C
   ///  * TypeRhs(Path, s, EE)
   ///    Here, Path must denote a type and s is a string that denotes the method/constructor Init
   ///      -- represents new Path.s(EE)
