Test/dafny0/DisplayExpressions.dfy
@@ -2,20 +2,25 @@
 // RUN: %diff "%s.expect" "%t"
 method M()
 {
-  var m := map[];
+  var m := map[];  // error: underspecified type
 }
 
 method N()
 {
-  var n := multiset{};
+  var n := multiset{};  // error: underspecified type
 }
 
 method O()
 {
-  var o := [];
+  var o := [];  // error: underspecified type
 }
 
 method P()
 {
-  var p := {};
+  var p := {};  // error: underspecified type
+}
+
+method Q()
+{
+  assert (((map[]))) == (((((map[])))));  // error (but not 10 errors)
 }
